CAT/rmonad_gen.v
@@ -56,7 +56,7 @@ Section gen_RMonad_Hom_struct.
 Variable tau : forall (c : obC), morD' (G2 (P c)) (Q (G1 c)).
 
 
-Class gen_RMonad_Hom_struct := {
+Class colax_RMonad_Hom_struct := {
   gen_rmonad_hom_rweta : forall c : obC,
          N _ ;; #G2 (rweta c) ;; tau c == rweta (G1 c) ;
   gen_rmonad_hom_rkl : forall (c d : obC) (f : morD (F c) (P d)),
@@ -67,9 +67,9 @@ Class gen_RMonad_Hom_struct := {
 
 Section Monad_Hom_NT.
 
-Variable M : gen_RMonad_Hom_struct.
+Variable M : colax_RMonad_Hom_struct.
 
-Program Instance gen_RMonad_Hom_NatTrans : 
+Program Instance colax_RMonad_Hom_NatTrans : 
     NT_struct (F:=CompF (RMFunc P) G2) 
              (G:=CompF G1 (RMFunc Q))
              (fun c => tau c).
@@ -78,7 +78,7 @@ Proof.
   simpl;
   intros c d f.
   unfold rlift.
-  assert (H':=gen_rmonad_hom_rkl (gen_RMonad_Hom_struct := M)).
+  assert (H':=gen_rmonad_hom_rkl (colax_RMonad_Hom_struct := M)).
   rewrite H'.
   apply praecomp.
   apply rkleisli_oid.
@@ -89,25 +89,25 @@ Proof.
   simpl in *.
   rewrite assoc.
   rewrite FComp.
-  assert (H:= gen_rmonad_hom_rweta (gen_RMonad_Hom_struct := M)).
+  assert (H:= gen_rmonad_hom_rweta (colax_RMonad_Hom_struct := M)).
   rewrite <- H.
   repeat rewrite <- assoc.
   rewrite HN.
   apply hom_refl.
 Qed.
 
-Definition gen_RMonad_Hom_NT := Build_NT gen_RMonad_Hom_NatTrans.
+Definition colax_RMonad_Hom_NT := Build_NT colax_RMonad_Hom_NatTrans.
 
 End Monad_Hom_NT.
 
 End gen_RMonad_Hom_struct.
 
-Record gen_RMonad_Hom := {
+Record colax_RMonad_Hom := {
 (*  Gone : Functor C C' ;
   Gtwo : Functor D D' ;*)
 (*  GOGT : NT (CompF G1 F') (CompF F G2) ;*)
   gen_rmonad_hom :> forall (c : obC), morD' (G2 (P c)) (Q (G1 c)) ;
-  gen_rmonad_hom_struct :> gen_RMonad_Hom_struct  gen_rmonad_hom
+  gen_rmonad_hom_struct :> colax_RMonad_Hom_struct  gen_rmonad_hom
 }.
 
 
@@ -131,13 +131,13 @@ Obligation Tactic := cat.
 Program Instance NT_i : NT_struct (F:=F O Id C) (G:= Id D O F)
         (fun c => id _ ).
 
-Program Instance gen_RMonad_Hom_id_s : gen_RMonad_Hom_struct 
+Program Instance colax_RMonad_Hom_id_s : colax_RMonad_Hom_struct 
      (P:=P)(Q:=P)(G1:=Id _ )(G2:=Id _ )
      (Build_NT NT_i)
      (fun c => id _ ).
 
-Definition gen_RMonad_Hom_id :=
-    Build_gen_RMonad_Hom gen_RMonad_Hom_id_s.
+Definition colax_RMonad_Hom_id :=
+    Build_colax_RMonad_Hom colax_RMonad_Hom_id_s.
 
 
 Variables obC' obD' obC'' obD'': Type.
@@ -164,8 +164,8 @@ Variable G2T : Functor D' D''.
 Variable NTT : NT (F'' O G1T) (G2T O F').
 
 
-Variable S : gen_RMonad_Hom P Q NS.
-Variable T : gen_RMonad_Hom Q R NTT.
+Variable S : colax_RMonad_Hom P Q NS.
+Variable T : colax_RMonad_Hom Q R NTT.
 
 Program Instance NT_c : 
 NT_struct (F:=F'' O (G1T O G1S)) (G:=(G2T O G2S) O F)
@@ -188,7 +188,7 @@ Proof.
 Qed.
 
  
-Program Instance gen_RMonad_Hom_comp_s : gen_RMonad_Hom_struct
+Program Instance colax_RMonad_Hom_comp_s : colax_RMonad_Hom_struct
   (P:=P) (Q:=R) (G1:=CompF 
                       (G1S)
                       (G1T)) 
@@ -199,8 +199,8 @@ Program Instance gen_RMonad_Hom_comp_s : gen_RMonad_Hom_struct
                 (fun c => #(G2T) (S c) ;; T (G1S c)).
 Next Obligation.
 Proof.
-  assert (H:=gen_rmonad_hom_rweta (gen_RMonad_Hom_struct := T)).
-  assert (H':=gen_rmonad_hom_rweta (gen_RMonad_Hom_struct := S)).
+  assert (H:=gen_rmonad_hom_rweta (colax_RMonad_Hom_struct := T)).
+  assert (H':=gen_rmonad_hom_rweta (colax_RMonad_Hom_struct := S)).
   rewrite <- H.
   repeat rewrite  assoc.
   apply praecomp.
@@ -213,8 +213,8 @@ Proof.
 Qed.
 Next Obligation.
 Proof.
-  assert (H:=gen_rmonad_hom_rkl (gen_RMonad_Hom_struct := T)).
-  assert (H':=gen_rmonad_hom_rkl (gen_RMonad_Hom_struct := S)).
+  assert (H:=gen_rmonad_hom_rkl (colax_RMonad_Hom_struct := T)).
+  assert (H':=gen_rmonad_hom_rkl (colax_RMonad_Hom_struct := S)).
   rewrite <- assoc.
   rewrite <- assoc.
   rewrite <- FComp.
@@ -231,8 +231,8 @@ Proof.
   apply hom_refl.
 Qed.
 
-Definition gen_RMonad_Hom_comp :=
-    Build_gen_RMonad_Hom gen_RMonad_Hom_comp_s.
+Definition colax_RMonad_Hom_comp :=
+    Build_colax_RMonad_Hom colax_RMonad_Hom_comp_s.
 
 (** Pullback along S *)
 
@@ -244,7 +244,7 @@ Variable N : RModule Q E.
 
 Obligation Tactic := idtac.
 
-Program Instance gen_PbRMod_s : 
+Program Instance colax_PbRMod_s : 
   RModule_struct P E (fun c : obC => N (G1S c)) := {
    rmkleisli c d f := rmkleisli (RModule_struct := N)
          (NS c ;; #(G2S) f ;; S d)
@@ -264,7 +264,7 @@ Proof.
   apply (rmkl_eq N).
   repeat rewrite assoc.
   apply praecomp.
-  assert (H:= gen_rmonad_hom_rkl (gen_RMonad_Hom_struct := S)).
+  assert (H:= gen_rmonad_hom_rkl (colax_RMonad_Hom_struct := S)).
   rewrite FComp.
   repeat rewrite assoc.
   apply praecomp.
@@ -279,12 +279,12 @@ Proof.
   rewrite <- (rmkleta N).
   apply (rmkl_eq N).
   cat.
-  assert (H:= gen_rmonad_hom_rweta (gen_RMonad_Hom_struct := S)).
+  assert (H:= gen_rmonad_hom_rweta (colax_RMonad_Hom_struct := S)).
   simpl in *.
   apply H.
 Qed.
 
-Definition gen_PbRMod := Build_RModule gen_PbRMod_s.
+Definition colax_PbRMod := Build_RModule colax_PbRMod_s.
 
 End rmonad_hom_id_comp.
 
@@ -310,7 +310,7 @@ Variable G1 : Functor C C'.
 Variable G2 : Functor D D'.
 Variable T : NT (F' O G1) (G2 O F).
 
-Variable f : gen_RMonad_Hom P Q T.
+Variable f : colax_RMonad_Hom P Q T.
 
 
 Program Instance F_rmod_s : RModule_struct P _ (fun x => G2 (P x)) := {
@@ -337,8 +337,8 @@ Qed.
 
 Definition F_rmod := Build_RModule F_rmod_s.
 
-Program Instance gen_PbRMod_ind_Hom_s : RModule_Hom_struct
-    (M:=F_rmod) (N:=gen_PbRMod f Q) f.
+Program Instance colax_PbRMod_ind_Hom_s : RModule_Hom_struct
+    (M:=F_rmod) (N:=colax_PbRMod f Q) f.
 Next Obligation.
 Proof.
   simpl.
@@ -348,8 +348,8 @@ Proof.
   apply f.
 Qed.
 
-Definition gen_PbRMod_ind_Hom := 
-   Build_RModule_Hom gen_PbRMod_ind_Hom_s.
+Definition colax_PbRMod_ind_Hom := 
+   Build_RModule_Hom colax_PbRMod_ind_Hom_s.
 
 
 Variable obE : Type.
@@ -361,30 +361,30 @@ Variable N N' : RMOD Q E.
 
 Obligation Tactic := cat.
 
-Program Instance gen_PROD_PM_s : RModule_Hom_struct 
-        (M:=product (C:=RMOD P E) (gen_PbRMod f N) (gen_PbRMod f N'))
-        (N:=gen_PbRMod f (product (C:=RMOD Q E) N N'))
+Program Instance colax_PROD_PM_s : RModule_Hom_struct 
+        (M:=product (C:=RMOD P E) (colax_PbRMod f N) (colax_PbRMod f N'))
+        (N:=colax_PbRMod f (product (C:=RMOD Q E) N N'))
         (fun c => id (product (N (G1 c)) (N' (G1 c)))).
 
-Definition gen_PROD_PM : 
-     product (C:=RMOD P E) (gen_PbRMod f N) (gen_PbRMod f N') ---> 
-            gen_PbRMod f (product (C:=RMOD Q E) N N') :=
-      Build_RModule_Hom gen_PROD_PM_s.
+Definition colax_PROD_PM : 
+     product (C:=RMOD P E) (colax_PbRMod f N) (colax_PbRMod f N') ---> 
+            colax_PbRMod f (product (C:=RMOD Q E) N N') :=
+      Build_RModule_Hom colax_PROD_PM_s.
 
 Variable h : N ---> N'.
 
 Obligation Tactic := rmonad.
 
-Program Instance gen_PbRMod_Hom_s : RModule_Hom_struct 
-     (M:=gen_PbRMod f N) (N:=gen_PbRMod f N') (fun c => h (G1 c)).
+Program Instance colax_PbRMod_Hom_s : RModule_Hom_struct 
+     (M:=colax_PbRMod f N) (N:=colax_PbRMod f N') (fun c => h (G1 c)).
 
-Definition gen_PbRMod_Hom : gen_PbRMod f N ---> gen_PbRMod f N' :=
-       Build_RModule_Hom gen_PbRMod_Hom_s.
+Definition colax_PbRMod_Hom : colax_PbRMod f N ---> colax_PbRMod f N' :=
+       Build_RModule_Hom colax_PbRMod_Hom_s.
 
 End pb_prod_func_and_Pb_ind_Hom.
 
-Coercion gen_RMonad_Hom_NatTrans : gen_RMonad_Hom_struct >-> NT_struct.
-Coercion gen_RMonad_Hom_NT : gen_RMonad_Hom_struct >-> NT.
+Coercion colax_RMonad_Hom_NatTrans : colax_RMonad_Hom_struct >-> NT_struct.
+Coercion colax_RMonad_Hom_NT : colax_RMonad_Hom_struct >-> NT.
 
 Implicit Arguments gen_rmonad_hom_rweta
 [obC obD obC' obD' morC morD morC' morD' C D C' D' F
